platform/cito/SetModule.v
@@ -10,19 +10,19 @@ Module Type Set_ (Key : MiniDecidableType).
 
   Parameter union : set -> set -> set.
 
-  Parameter union_has_left : forall a b x, mem x a -> mem x (union a b).
+  Parameter union_correct : forall a b x, mem x (union a b) <-> mem x a \/ mem x b.
 
-  Parameter union_has_right : forall a b x, mem x b -> mem x (union a b).
+  Parameter diff : set -> set -> set.
 
-  Parameter union_elim : forall a b x, mem x (union a b) -> mem x a \/ mem x b.
+  Parameter diff_correct : forall a b x, mem x (diff a b) <-> mem x a /\ ~ mem x b.
 
   Parameter empty : set.
 
   Parameter empty_correct : forall x, ~ mem x empty.
 
-  Parameter add : set -> Key.t -> set.
+  Parameter singleton : Key.t -> set.
 
-  Parameter add_added : forall s x, mem x (add s x).
+  Parameter singleton_correct : forall x x', mem x' (singleton x) <-> x' = x.
 
 End Set_.
 
@@ -36,9 +36,11 @@ End MembershipDecidableSet.
 
 Module Notations (Key : MiniDecidableType) (Import S : Set_ Key).
   Delimit Scope set_scope with set.
-  Infix "%in" := mem (at level 60): set_scope.
+  Infix "^" := mem : set_scope.
   Infix "+" := union : set_scope.
-  Notation "{}" := empty : set_scope.
+  Infix "-" := diff : set_scope.
+  Notation "0" := empty : set_scope.
+  Notation "!" := singleton : set_scope.
 End Notations.
 
 Module Relations (Key : MiniDecidableType) (Import S : Set_ Key).
@@ -46,38 +48,63 @@ Module Relations (Key : MiniDecidableType) (Import S : Set_ Key).
   Definition subset (a b : set) := forall x, mem x a -> mem x b.
   Infix "<=" := subset : set_scope.
 
-  Lemma subset_correct : forall a b, subset a b -> forall x, mem x a -> mem x b.
-    eauto.
+  Lemma subset_correct : forall a b, subset a b <-> forall x, mem x a -> mem x b.
+    intuition.
   Qed.
 
-  Definition subset_refl : forall s, subset s s.
+  Lemma subset_refl : forall s, subset s s.
     unfold subset; intuition.
   Qed.
 
-  Definition subset_union_2 : forall a b, subset a (union a b).
-    unfold subset; intros; eapply union_has_left; eauto.
-  Qed.
-  
-  Definition subset_union_1 : forall a b, subset a (union b a).
-    unfold subset; intros; eapply union_has_right; eauto.
+  Lemma subset_trans : forall a b c, subset a b -> subset b c -> subset a c.
+    unfold subset; intuition.
   Qed.
 
-  Definition union_same_subset : forall s, subset (union s s) s.
-    unfold subset; intros; eapply union_elim in H; destruct H; eauto.
+  Lemma subset_union_left : forall a b, subset a (union a b).
+    unfold subset; intros; eapply union_correct; eauto.
+  Qed.
+  
+  Lemma subset_union_right : forall a b, subset b (union a b).
+    unfold subset; intros; eapply union_correct; eauto.
+  Qed.
+
+  Lemma union_subset : forall (a b c : set), subset a c -> subset b c -> subset (union a b) c.
+    unfold subset; intros; eapply union_correct in H1; destruct H1; eauto.
+  Qed.
+
+  Lemma union_same_subset : forall s, subset (union s s) s.
+    intros; eapply union_subset; eapply subset_refl.
+  Qed.
+
+  Lemma subset_union_same : forall s, subset s (union s s).
+    intros; eapply subset_union_left.
+  Qed.
+
+  Lemma diff_subset : forall a b, subset (diff a b) a.
+    unfold subset; intros; eapply diff_correct in H; intuition.
   Qed.
 
 End Relations.
 
-Module Singleton (Key : MiniDecidableType) (Import S : Set_ Key).
+Module Util (Key : MiniDecidableType) (Import S : Set_ Key).
 
-  Definition singleton x := add empty x.
-  Notation "{ x }" := (singleton x) : set_scope.
-
-  Lemma singleton_mem : forall x, mem x (singleton x).
-    unfold singleton; intros; eapply add_added.
+  Lemma union_elim : forall a b x, mem x (union a b) -> mem x a \/ mem x b.
+    intros; eapply union_correct in H; eauto.
   Qed.
 
-End Singleton.
+  Lemma union_intro : forall a b x, mem x a \/ mem x b -> mem x (union a b).
+    intros; eapply union_correct; eauto.
+  Qed.
+
+  Lemma mem_union_left : forall a b x, mem x a -> mem x (union a b).
+    intros; eapply union_intro; intuition.
+  Qed.
+
+  Lemma mem_union_right : forall a b x, mem x b -> mem x (union a b).
+    intros; eapply union_intro; intuition.
+  Qed.
+
+End Util.
 
 (* Implementations *)
 
@@ -89,36 +116,31 @@ Module ArrowSet (Key : MiniDecidableType) <: MembershipDecidableSet Key.
 
   Definition union (a b : set) := fun x => orb (a x) (b x).
 
-  Lemma union_has_left : forall a b x, mem x a -> mem x (union a b).
-    unfold mem, union; intuition.
+  Lemma union_correct : forall a b x, mem x (union a b) <-> mem x a \/ mem x b.
+    unfold mem, union; intuition; eapply Bool.orb_true_elim in H; destruct H; intuition.
   Qed.
 
-  Lemma union_has_right : forall a b x, mem x b -> mem x (union a b).
-    unfold mem, union; intuition.
+  Definition diff (a b : set) := fun x => andb (a x) (negb (b x)).
+
+  Lemma diff_correct : forall a b x, mem x (diff a b) <-> mem x a /\ ~ mem x b.
+    unfold mem, diff; intuition; eapply Bool.andb_true_iff in H; destruct H; intuition; rewrite H0 in H1; intuition.
   Qed.
 
-  Lemma union_elim : forall a b x, mem x (union a b) -> mem x a \/ mem x b.
-    unfold mem, union.
-    intros.
-    eapply Bool.orb_true_elim in H.
-    destruct H; intuition.
-  Qed.
-  
   Definition empty : set := fun _ => false.
 
   Lemma empty_correct : forall x, ~ mem x empty.
     unfold empty, mem; eauto.
   Qed.
 
-  Definition add (s : set) x : set :=
+  Definition singleton x := 
     fun x' =>
       if Key.eq_dec x' x then
         true
       else
-        s x'.
+        false.
 
-  Lemma add_added : forall s x, mem x (add s x).
-    unfold add, mem; intros; destruct (Key.eq_dec x x); eauto.
+  Lemma singleton_correct : forall x x', mem x' (singleton x) <-> x' = x.
+    unfold mem, singleton; intros; destruct (Key.eq_dec x' x); intuition; intuition; discriminate.
   Qed.
 
   Definition mem_dec : forall x s, {mem x s} + {~ mem x s}.
@@ -127,7 +149,6 @@ Module ArrowSet (Key : MiniDecidableType) <: MembershipDecidableSet Key.
 
   Include Notations Key.
   Include Relations Key.
-  Include Singleton Key.
+  Include Util Key.
 
 End ArrowSet.
-
